Get Local.v compiling.

src/rocq/Handlers/Local.v
@@ -7,18 +7,21 @@ From ExtLib Require Import
   Structures.Monads
   Structures.Maps.
 
-From ITree Require Import
-  ITree
-  Eq.Eqit
-  Events.State
-  Events.StateFacts.
-
 From Vellvm Require Import
   Utils.Util
   Utils.Error
   Utils.Tactics
   Semantics.LLVMEvents
   Semantics.Memory.Sizeof.
+
+Unset Universe Checking.
+From CTree Require Import
+  CTree
+  Fold
+  FoldCTree
+  FoldStateT
+  Eq
+  SBisim.
 
 Require Import Ceres.Ceres.
 
@@ -27,6 +30,7 @@ Set Contextual Implicit.
 
 Import MonadNotation.
 Import ITree.Basics.Basics.Monads.
+Import CategoryOps.
 Open Scope string_scope.
 (* end hide *)
 
@@ -39,7 +43,7 @@ Section Locals.
   Context {map : Type}.
   Context {M: Map k v map}.
   Context {SK : Serialize k}.
-  Definition handle_local {E} `{FailureE -< E} : (LocalE k v) ~> stateT map (itree E) :=
+  Definition handle_local {E BR} `{FailureE -< E} : (LocalE k v) ~> stateT map (ctree E BR) :=
     fun _ e env =>
       match e with
       | LocalWrite k v => ret (Maps.add k v env, tt)
@@ -52,60 +56,60 @@ Section Locals.
 
   Open Scope monad_scope.
   Section PARAMS.
-    Variable (E F G H: Type -> Type).
+    Variable (E F G H BR: Type -> Type).
     Context `{FailureE -< G}.
     Notation Effin := (E +' F +' (LocalE k v) +' G).
     Notation Effout := (E +' F +' G).
 
-    Definition E_trigger {M} : forall R, E R -> (stateT M (itree Effout) R) :=
+    Definition E_trigger {M} : forall R, E R -> (stateT M (ctree Effout BR) R) :=
       fun R e m => r <- trigger e ;; ret (m, r).
 
-    Definition F_trigger {M} : forall R, F R -> (stateT M (itree Effout) R) :=
+    Definition F_trigger {M} : forall R, F R -> (stateT M (ctree Effout BR) R) :=
       fun R e m => r <- trigger e ;; ret (m, r).
 
-    Definition G_trigger {M} : forall R , G R -> (stateT M (itree Effout) R) :=
+    Definition G_trigger {M} : forall R , G R -> (stateT M (ctree Effout BR) R) :=
       fun R e m => r <- trigger e ;; ret (m, r).
 
     Definition interp_local_h := (case_ E_trigger (case_ F_trigger (case_ handle_local G_trigger))).
-    Definition interp_local : itree Effin ~> stateT map (itree Effout) :=
+    Definition interp_local : ctree Effin BR ~> stateT map (ctree Effout BR) :=
       interp_state interp_local_h.
 
 
     Section Structural_Lemmas.
 
       Lemma interp_local_bind :
-        forall (R S : Type) (t : itree Effin R) (k : R -> itree Effin S) s,
-          interp_local (ITree.bind t k) s ≅
-                       ITree.bind (interp_local t s) (fun '(s',r) => interp_local (k r) s').
+        forall (R S : Type) (t : ctree Effin BR R) (k : R -> ctree Effin BR S) s,
+          interp_local (CTree.bind t k) s ≅
+                       CTree.bind (interp_local t s) (fun '(s',r) => interp_local (k r) s').
       Proof using.
         intros.
         unfold interp_local.
         setoid_rewrite interp_state_bind.
-        apply eq_itree_clo_bind with (UU := Logic.eq).
+        apply equ_clo_bind_eq.
+        intros (?&?).
         reflexivity.
-        intros [] [] EQ; inversion EQ; reflexivity.
       Qed.
 
       Lemma interp_local_ret :
         forall (R : Type) l (x: R),
-          interp_local (Ret x: itree Effin R) l ≅ Ret (l,x).
+          interp_local (Ret x: ctree Effin BR R) l ≅ Ret (l,x).
       Proof using.
         intros; apply interp_state_ret.
       Qed.
 
-      Lemma interp_local_Tau :
-        forall {R} (t: itree Effin R) l,
-          interp_local (Tau t) l ≅ Tau (interp_local t l).
+      Lemma interp_local_guard :
+        forall {R} (t: ctree Effin BR R) l,
+          interp_local (Guard t) l ≅ Guard (interp_local t l).
       Proof using.
         intros.
-        unfold interp_local; rewrite interp_state_tau; reflexivity.
+        unfold interp_local; rewrite interp_state_guard; reflexivity.
       Qed.
 
       Lemma interp_local_vis_eqit:
         forall (g : map) S X
-          (kk : X -> itree Effin S)
+          (kk : X -> ctree Effin BR S)
           (e : Effin X),
-          interp_local (Vis e kk) g ≅ ITree.bind (interp_local_h e g) (fun (sx : map * X) => Tau (interp_local (kk (snd sx)) (fst sx))).
+          interp_local (Vis e kk) g ≅ CTree.bind (interp_local_h e g) (fun (sx : map * X) => Guard (interp_local (kk (snd sx)) (fst sx))).
       Proof using.
         intros.
         unfold interp_local.
@@ -114,28 +118,30 @@ Section Locals.
       Qed.
 
       Lemma interp_local_vis:
-        forall (g : map) S X (kk : X -> itree Effin S) (e : Effin X),
-          interp_local (Vis e kk) g ≈ ITree.bind (interp_local_h e g) (fun (sx : map * X) => interp_local (kk (snd sx)) (fst sx)).
+        forall (g : map) S X (kk : X -> ctree Effin BR S) (e : Effin X),
+          interp_local (Vis e kk) g ~ CTree.bind (interp_local_h e g) (fun (sx : map * X) => interp_local (kk (snd sx)) (fst sx)).
       Proof using.
         intros.
         rewrite interp_local_vis_eqit.
-        apply eutt_eq_bind.
-        intros ?; tau_steps; reflexivity.
+        upto_bind_eq.
+        intros ?; rewrite sb_guard; reflexivity.
       Qed.
 
       Lemma interp_local_trigger:
         forall (g : map) X (e : Effin X),
-          interp_local (ITree.trigger e) g ≈ interp_local_h e g.
+          interp_local (CTree.trigger e) g ~ interp_local_h e g.
       Proof using.
         intros.
         unfold interp_local.
         rewrite interp_state_trigger.
+        setoid_rewrite sb_guard.
+        setoid_rewrite bind_ret_r.
         reflexivity.
       Qed.
 
       Lemma interp_local_bind_trigger_eqit:
-        forall (g : map) S X (kk : X -> itree Effin S) (e : Effin X),
-          interp_local (ITree.bind (trigger e) kk) g ≅ ITree.bind (interp_local_h e g) (fun (sx : map * X) => Tau (interp_local (kk (snd sx)) (fst sx))).
+        forall (g : map) S X (kk : X -> ctree Effin BR S) (e : Effin X),
+          interp_local (CTree.bind (trigger e) kk) g ≅ CTree.bind (interp_local_h e g) (fun (sx : map * X) => Guard (interp_local (kk (snd sx)) (fst sx))).
       Proof using.
         intros.
         unfold interp_local.
@@ -145,32 +151,35 @@ Section Locals.
       Qed.
 
       Lemma interp_local_trigger_bind:
-        forall (g : map) S X (kk : X -> itree Effin S) (e : Effin X),
-          interp_local (ITree.bind (trigger e) kk) g ≈ ITree.bind (interp_local_h e g) (fun (sx : map * X) => interp_local (kk (snd sx)) (fst sx)).
+        forall (g : map) S X (kk : X -> ctree Effin BR S) (e : Effin X),
+          interp_local (CTree.bind (trigger e) kk) g ~ CTree.bind (interp_local_h e g) (fun (sx : map * X) => interp_local (kk (snd sx)) (fst sx)).
       Proof using.
         intros.
         rewrite interp_local_bind_trigger_eqit.
-        apply eutt_eq_bind.
-        intros ?; tau_steps; reflexivity.
+        upto_bind_eq.
+        intros ?; rewrite sb_guard; reflexivity.
       Qed.
 
-      #[global] Instance Proper_interp_local {T} {b} :
-        Proper (eqit eq b b ==> Monad.eq1) (@interp_local T).
+      #[global] Instance Proper_interp_local_equ {T} :
+        Proper (equ eq  ==> eq ==> equ eq) (@interp_local T).
       Proof.
-        intros ? ? ?.
-        do 3 red.
-        intros a.
-        do 2 red.
-        destruct b; try setoid_rewrite H1; try reflexivity.
+        intros ? ? ? ? ? ?; subst.
+        rewrite H1.
+        reflexivity.
       Qed.
 
-      #[global] Instance Proper_interp_local_pointwise {T} {b} :
-        Proper (eqit eq b b ==> eq ==> eqit eq b b) (@interp_local T).
+      #[global] Instance Proper_interp_local_sbisim {T} :
+        Proper (sbisim eq  ==> eq ==> sbisim eq) (@interp_local T).
+      Proof.
+        intros ? ? ? ? ? ?; subst.
+      Abort.
+
+      #[global] Instance Proper_interp_local_pointwise_equ {T} :
+        Proper (equ eq  ==> eq ==> equ eq) (@interp_local T).
       Proof.
         intros ? ? ? ? ? ?; subst.
         unfold interp_local.
-        destruct b; rewrite H1;
-          reflexivity.
+        rewrite H1; reflexivity.
       Qed.
 
     End Structural_Lemmas.
